lib/Lib_List.v
@@ -18,16 +18,19 @@ Definition l : vsymbol := ("l", list).
 
 (*Basic theory of Polymorphic Lists*)
 
+(*Function definitions separately makes context nicer*)
+Definition is_nil_body : formula := <f
+  match {l} : list with
+  | Nil<a> nil -> true
+  | Cons<a>(_, _) -> false
+  end
+  f>.
+
 Definition List : theory :=
   rev [
     (*TODO: notations would be nice*)
     tdef (datatype_def list_mut);
-    tdef (nonrec_pred is_nil [l] <f
-      match {l} : list with
-      | Nil<a> nil -> true
-      | Cons<a>(_, _) -> false
-      end
-    f>);
+    tdef (nonrec_pred is_nil [l] is_nil_body);
     (*We don't have "ensures"*)
     tprop Plemma "is_nil_spec" <f forall l,
       is_nil<a>({l}) <-> [list] {l} = Nil<a>() f>
@@ -36,22 +39,122 @@ Definition List : theory :=
 (*Length of a list*)
 Definition length : funsym := funsym_noty "length" [list] vty_int.
 Definition r : vsymbol := ("r", list).
+
+Definition length_body : term :=  <t
+  match {l} : list with
+  | Nil<a> nil -> Int.zero()
+  | Cons<a>(_, {r}) -> Int.plus(Int.one(), length<a>({r}))
+  end
+  t>.
+
 Definition Length : theory :=
   rev [
     tuse Int.Int false;
     tuse List false;
-    tdef (rec_fun length [l] <t
-      match {l} : list with
-      | Nil<a> nil -> Int.zero()
-      | Cons<a>(_, {r}) -> Int.plus(Int.one(), length<a>({r}))
-      end
-    t>);
+    tdef (rec_fun length [l] length_body);
     tprop Plemma "Length_nonnegative" <f forall l,
       Int.ge(length<a>({l}), Int.zero()) f>;
     tprop Plemma "Length_nil" <f forall l,
       [vty_int] length<a>({l}) = Int.zero() <-> [list] {l} = Nil<a>()
     f>
   ].
+
+(*Membership in a list*)
+Definition mem : predsym := predsym_noty "mem" [a; list].
+Definition x: vsymbol :=("x", a).
+Definition y: vsymbol := ("y", a).
+
+Definition mem_body : formula := <f
+  match {l} : list with
+  | Nil<a> nil -> false
+  | Cons<a>({y}, {r}) -> [a] {x} = {y} \/ mem<a>({x}, {r})
+  end
+  f>.
+
+Definition Mem : theory :=
+  rev [
+    tuse List false;
+    tdef (rec_pred mem [x; l] mem_body)
+  ].
+
+(*Appending two lists*)
+Definition app : funsym := binop "app" list.
+Definition l1 : vsymbol := ("l1", list).
+Definition l2 : vsymbol := ("l2", list).
+Definition l3 : vsymbol := ("l3", list).
+Definition app_body : term := <t
+match {l1} : list with
+| Nil<a> nil -> {l2}
+| Cons<a>({y}, {r}) -> Cons<a>({y}, app<a>({r}, {l2}))
+end
+t>.
+
+(*This involves lots of things: list, length, int, mem, 
+  and new definitions.
+  Can the automation handle this?*)
+Definition Append : theory :=
+  rev [
+    tuse List false;
+    tdef (rec_fun app [l1; l2] app_body);
+    tprop Plemma "Append_assoc" <f forall l1, forall l2, forall l3,
+      [list] app<a>({l1}, app<a>({l2}, {l3})) =
+             app<a>(app<a>({l1}, {l2}), {l3})
+      f>;
+    tprop Plemma "Append_l_nil" <f forall l1,
+      [list] app<a>({l1}, Nil<a>()) = {l1} f>;
+    (*TODO: change so import order doesn't matter as much*)
+    tuse Int.Int false;
+    tuse Length false;
+    tprop Plemma "Append_length" <f forall l1, forall l2,
+      [vty_int] length<a>(app<a>({l1}, {l2})) =
+        Int.plus(length<a>({l1}), length<a>({l2})) f>;
+    tuse Mem false;
+    tprop Plemma "mem_append" <f forall x, forall l1, forall l2,
+      mem<a>({x}, app<a>({l1}, {l2})) <->
+      mem<a>({x}, {l1}) \/ mem<a>({x}, {l2}) f>;
+    (*NOTE: likely not proving this one*)
+    tprop Plemma "mem_decomp" <f forall x, forall l1,
+      mem<a>({x}, {l1}) ->
+      exists l2, exists l3, 
+        [list] {l1} = app<a>({l2}, Cons<a>({x}, {l3})) f>
+  ].
+
+(*Reversing a list*)
+Definition reverse : funsym := unop "reverse" list.
+Definition reverse_body : term := <t
+match {l} : list with
+| Nil<a> nil -> Nil<a>()
+| Cons<a>({x}, {r}) -> 
+    app<a>(reverse<a>({r}), Cons<a>({x}, Nil<a>()))
+end
+t>.
+
+Definition Reverse : theory :=
+  rev [
+    tuse List false;
+    (*NOTE: why3 only requires Append, our system is more
+      limited so we need Int and Length here*)
+    tuse Int.Int false;
+    tuse Length false;
+    tuse Mem false;
+    tuse Append false;
+    tdef (rec_fun reverse [l] reverse_body);
+    tprop Plemma "reverse_append" <f forall l1, forall l2, forall x,
+      [list] app<a>(reverse<a>(Cons<a>({x}, {l1})), {l2}) =
+        app<a>(reverse<a>({l1}), Cons<a>({x}, {l2})) f>;
+    tprop Plemma "reverse_cons" <f forall l, forall x,
+      [list] reverse<a>(Cons<a>({x}, {l})) =
+        app<a>(reverse<a>({l}), Cons<a>({x}, Nil<a>())) f>;
+    tprop Plemma "cons_reverse" <f forall l, forall x,
+      [list] Cons<a>({x}, reverse<a>({l})) =
+        reverse<a>(app<a>({l}, Cons<a>({x}, Nil<a>()))) f>;
+    tprop Plemma "reverse_reverse" <f forall l,
+      [list] reverse<a>(reverse<a>({l})) = {l} f>;
+    tprop Plemma "reverse_mem" <f forall l, forall x,
+      mem<a>({x}, {l}) <-> mem<a>({x}, reverse<a>({l})) f>;
+    tprop Plemma "Reverse_length" <f forall l,
+      [vty_int] length<a>(reverse<a>({l})) = length<a>({l}) f>
+  ].  
 
 (*Plan:
 write down:
