lib/Verif_List.v
@@ -1,5 +1,6 @@
 Require Import StdLib.
 Require Import Lib_List.
+Set Bullet Behavior "Strict Subproofs".
 
 (*First, just do typechecking*)
 Lemma list_typed : typed_theory List.List.
@@ -11,3 +12,275 @@ Lemma length_typed : typed_theory List.Length.
 Proof.
   check_theory.
 Qed.
+
+Lemma mem_typed : typed_theory List.Mem.
+Proof. 
+  check_theory.
+Qed.
+
+Lemma app_typed: typed_theory List.Append.
+Proof.
+  check_theory.
+Qed.
+
+Lemma reverse_typed: typed_theory List.Reverse.
+Proof.
+  check_theory.
+Qed.
+
+(*Contexts*)
+Module ListCtx.
+
+Import Lib_Relations.Relations.
+Import Lib_Algebra.Algebra.
+Import Lib_Int.Int.
+Import Lib_List.List.
+
+Lemma list_ctx : theory_ctx_ext List = 
+[:: nonrec_pred is_nil [:: l] is_nil_body; datatype_def list_mut].
+Proof.
+  reflexivity.
+Qed.
+
+Lemma length_ctx : theory_ctx_ext Length = [:: rec_fun length [:: l] length_body].
+Proof.
+  reflexivity.
+Qed.
+
+Lemma mem_ctx: theory_ctx_ext Mem = [:: rec_pred mem [:: x; l] mem_body].
+Proof.
+  reflexivity.
+Qed.
+
+Lemma app_ctx: theory_ctx_ext Append = [:: rec_fun app [:: l1; l2] app_body].
+Proof.
+  reflexivity.
+Qed.
+
+Lemma reverse_ctx: theory_ctx_ext Reverse = [:: rec_fun reverse [:: l] reverse_body].
+Proof.
+  reflexivity.
+Qed.
+
+End ListCtx.
+
+Module ListAxioms.
+
+Import Lib_Relations.Relations.
+Import Lib_Algebra.Algebra.
+Import Lib_Int.Int.
+Import Lib_List.List.
+
+Lemma list_axioms : theory_axioms_ext List = 
+[:: ("is_nil_spec", <f forall l,
+      is_nil<a>({l}) <-> [list] {l} = Nil<a>() f>)].
+Proof.
+  reflexivity.
+Qed.
+
+Lemma length_axioms : theory_axioms_ext Length =
+[("Length_nil", <f forall l,
+    [vty_int] length<a>({l}) = zero() <-> [list] {l} = Nil<a>()
+    f>);
+  ("Length_nonnegative", <f forall l,
+    ge(length<a>({l}), zero()) f>)].
+Proof.
+  reflexivity.
+Qed.
+
+Lemma mem_axioms: theory_axioms_ext Mem = nil.
+Proof. 
+  reflexivity.
+Qed.
+
+Lemma app_axioms: theory_axioms_ext Append =
+[
+  ("mem_decomp",
+  <f forall x, forall l1,
+    mem<a>({x}, {l1}) ->
+    exists l2, exists l3, 
+      [list] {l1} = app<a>({l2}, Cons<a>({x}, {l3})) f>);
+  ("mem_append", 
+  <f forall x, forall l1, forall l2,
+    mem<a>({x}, app<a>({l1}, {l2})) <->
+    mem<a>({x}, {l1}) \/ mem<a>({x}, {l2}) f>);
+  ("Append_length", 
+  <f forall l1, forall l2,
+    [vty_int] length<a>(app<a>({l1}, {l2})) =
+      plus(length<a>({l1}), length<a>({l2})) f>);
+  ("Append_l_nil", <f forall l1,
+    [list] app<a>({l1}, Nil<a>()) = {l1} f>);
+  ("Append_assoc", <f forall l1, forall l2, forall l3,
+    [list] app<a>({l1}, app<a>({l2}, {l3})) =
+          app<a>(app<a>({l1}, {l2}), {l3})
+    f>)
+].
+Proof.
+  reflexivity.
+Qed.
+
+(*TODO: reverse axioms*)
+End ListAxioms.
+
+(*Helpful for lemmas*)
+Module OtherCtx.
+
+Import Lib_Relations.Relations.
+Import Lib_Algebra.Algebra.
+Import Lib_Int.Int.
+Import Lib_List.List.
+
+
+(*TODO: move*)
+Require Import Verif_Int.
+Lemma length_int_list_ctx:
+  (theory_ctx_ext Length ++
+   theory_ctx_ext Int ++
+   (rec_fun app [:: l1; l2] app_body :: (theory_ctx_ext List ++ [::])%list)%SEQ) =
+[:: rec_fun length [:: l] length_body;
+nonrec_pred ge [:: Lib_Int.Int.x; Lib_Int.Int.y] ge_body;
+nonrec_pred le [:: Lib_Int.Int.x; Lib_Int.Int.y] le_body;
+nonrec_pred gt [:: Lib_Int.Int.x; Lib_Int.Int.y] gt_body;
+nonrec_fun sub [:: Lib_Int.Int.x; Lib_Int.Int.y] sub_body; 
+abs_pred lt; abs_fun mult; abs_fun plus; abs_fun neg;
+nonrec_fun one [::] (Tconst (ConstInt 1));
+nonrec_fun zero [::] (Tconst (ConstInt 0)); rec_fun app [:: l1; l2] app_body;
+nonrec_pred is_nil [:: l] is_nil_body; datatype_def list_mut].
+Proof.
+  reflexivity.
+Qed.
+
+End OtherCtx.
+
+(*Prove lemmas*)
+
+Module ListProofs.
+
+Import Lib_Relations.Relations.
+Import Lib_Algebra.Algebra.
+Import Lib_Int.Int.
+Import Lib_List.List.
+
+Definition a_ : vty := tyconst "a".
+Definition x_ : vsymbol := ("x", a_).
+Definition y_ : vsymbol := ("y", a_).
+Definition list_a : vty := vty_cons list_ts [a_].
+Definition r_: vsymbol := ("r", list_a).
+Definition l1_ : vsymbol := ("l1", list_a).
+Definition l2_ : vsymbol := ("l2", list_a).
+Definition l3_ : vsymbol := ("l3", list_a).
+
+Definition l1__ : term := Tfun (constsym "l1" list_a) nil nil.
+Definition l2__ : term := Tfun (constsym "l2" list_a) nil nil.
+Definition l3__ : term := Tfun (constsym "l3" list_a) nil nil.
+Definition l__ : term := Tfun (constsym "l" list_a) nil nil.
+
+Ltac extra_simpl ::= fold a_; fold x_; fold y_; 
+  fold list_a;
+  fold l1_; fold l2_; fold l3_; fold r_;
+  unfold t_constsym;
+  fold l1__; fold l2__; fold l3__; fold l__;
+  repeat (tryif progress(unfold ty_subst; try unfold ty_subst_var)
+    then simpl else idtac).
+
+  Ltac wunfold_at x n :=
+  apply D_unfold_single with (f:=x)(i:=n); [prove_closed |];
+  unfold unfold_f_single; simpl; unfold unfold_f_single_aux; simpl;
+  unfold sub_fun_body_f, replace_tm_f, sub_body_t, safe_sub_ts; simpl;
+  repeat (progress(extra_simpl)).
+
+(*This is a hack, but unfolding the context
+  takes a long time. Instead we prove an equivalence*)
+
+
+(*Start with interesting ones (app, reverse)*)
+Lemma app_valid: valid_theory Append.
+Proof.
+  simpl valid_theory.
+  split_all; auto; exists ["a"].
+  5: {
+    (*[app] is associative*)
+    (*Let's expand the context but NOT the assumptions (delta)*)
+    apply soundness.
+    simpl_task.
+    rewrite ListCtx.list_ctx. simpl.
+    rewrite ListAxioms.list_axioms. simpl.
+    simpl_mono.
+    winduction.
+    - (*Nil case: simplify both sides*)
+      wintros "l2". wintros "l3".
+      wunfold_at app 0%N. 
+      wsimpl_match.
+      wunfold_at app 2%N.
+      wsimpl_match.
+      wreflexivity.
+    - wintros "x" "l" "IH" "l2" "l3".
+      wunfold_at app 0%N.
+      wsimpl_match.
+      wunfold_at app 3%N.
+      wsimpl_match.
+      wunfold_at app 2%N.
+      wsimpl_match.
+      (*Now we can rewrite with the IH*)
+      wf_equal. wreflexivity.
+      wspecialize "IH" l2__ l3__.
+      wrewrite "IH".
+      wreflexivity.
+  }
+  4: {
+    (*l ++ nil = l*)
+    (*This proof is much easier, it is almost the same
+      as in Coq*)
+    apply soundness.
+    simpl_task.
+    rewrite ListCtx.list_ctx. simpl.
+    rewrite ListAxioms.list_axioms. simpl.
+    simpl_mono.
+    winduction.
+    - wunfold_at app 0%N. wsimpl_match.
+      wreflexivity.
+    - wintros "x" "l" "IH".
+      wunfold_at app 0%N. wsimpl_match.
+      wrewrite "IH".
+      wreflexivity.
+  }
+  3: {
+    (*length (l1 ++ l2) = length l1 + length l2*)
+    apply soundness.
+    simpl_task.
+    (*simplify context by rewriting because unfolding takes forever*)
+    rewrite ListCtx.length_ctx.
+    rewrite Verif_Int.IntCtx.int_ctx.
+    rewrite ListCtx.list_ctx. simpl.
+    (*Simplify delta*)
+    rewrite ListAxioms.length_axioms.
+    rewrite ListAxioms.list_axioms.
+    rewrite Verif_Int.IntCtx.int_axioms.
+    simpl.
+    simpl_mono.
+    winduction.
+    - wintros "l2". wunfold_at app 0%N. wsimpl_match.
+      wunfold_at length 1%N.
+      wsimpl_match.
+      (*Use fact that x + 0 = x*)
+      wspecialize "Unit_def_l" <t length<a_>(l2__) t>.
+      wrewrite "Unit_def_l".
+      wreflexivity.
+    - (*Inductive case*)
+      wintros "x" "l" "IH" "l2".
+      wunfold_at app 0%N; wsimpl_match.
+      wunfold_at length 0%N; wsimpl_match.
+      wunfold_at length 1%N; wsimpl_match.
+      (*Use IH+add assoc*)
+      wspecialize "IH" l2__.
+      wrewrite "IH".
+      wspecialize "Assoc" <t one() t> <t length<a_>(l__) t>
+        <t length<a_>(l2__) t>.
+      wrewrite "Assoc".
+      wreflexivity.
+  }
+  (*We do not (yet) do the mem goals*)
+  (*TODO: do predicate unfolding then this*)
+  admit.
+  admit.
+Admitted.
