lib/Verif_Int.v
@@ -10,3 +10,75 @@ Lemma int_valid: valid_theory Int.Int.
 Proof.
   simpl. auto.
 Qed.
+Require Import Verif_Algebra.
+Module IntCtx.
+(*Useful for avoiding unfolding*)
+
+Import Lib_Relations.Relations.
+Import Lib_Algebra.Algebra.
+Import Lib_Int.Int.
+
+Lemma int_ctx: 
+theory_ctx_ext Int.Int = 
+[:: nonrec_pred Int.ge [:: Int.x; Int.y] Int.ge_body;
+    nonrec_pred Int.le [:: Int.x; Int.y] Int.le_body;
+    nonrec_pred Int.gt [:: Int.x; Int.y] Int.gt_body;
+    nonrec_fun Int.sub [:: Int.x; Int.y] Int.sub_body; abs_pred Int.lt;
+    abs_fun Int.mult; abs_fun Int.plus; abs_fun Int.neg;
+    nonrec_fun Int.one [::] (Tconst (ConstInt 1));
+    nonrec_fun Int.zero [::] (Tconst (ConstInt 0))].
+Proof.
+  reflexivity.
+Qed.
+
+Definition z := ("z", vty_int).
+
+Lemma int_axioms:
+  theory_axioms_ext Int.Int = 
+  [("CompatOrderMult", <f 
+    forall x, forall y, forall z,
+    le({x}, {y}) -> le(zero(), {z}) -> 
+    le(mult({x}, {z}), mult({y}, {z})) f>);
+  ("CompatOrderAdd", <f forall x, forall y, forall z,
+      le({x}, {y}) -> le(plus({x}, {z}), plus({y}, {z})) f>);
+  ("ZeroLessOne", <f le (zero(), one()) f>);
+  ("Total", <f forall x, forall y,
+    le({x}, {y}) \/ le({y}, {x}) f>);
+  ("Antisymm", <f forall x, forall y,
+      le({x}, {y}) -> le({y}, {x}) -> [vty_int] {x} = {y} f>);
+  ("Trans", <f forall x, forall y, forall z, 
+      le ({x}, {y}) -> le ({y}, {z}) -> le({x}, {z}) f>);
+  ("Refl", <f forall x, le({x}, {x}) f>);
+  ("NonTrivialRing", <f ([vty_int] zero() != one()) f>);
+  ("Unitary", <f forall x, [vty_int] mult(one(), {x}) = {x} f>);
+  ("MulComm.Comm", <f
+    forall x, forall y, [vty_int] mult({x}, {y}) = mult({y}, {x}) f>);
+  ("Mul_distr_r", <f
+      forall x, forall y, forall z,
+        [vty_int] mult(plus({y}, {z}), {x}) = plus(mult({y}, {x}), mult({z}, {x}))
+    f>);
+  ("Mul_distr_l", <f
+    forall x, forall y, forall z, 
+      [vty_int] mult({x}, plus({y}, {z})) = plus(mult({x}, {y}), mult({x}, {z}))
+  f>);
+  ("MulAssoc.Assoc",
+      <f forall x, forall y, forall z, 
+        [vty_int] (mult (mult ({x}, {y}), {z})) = (mult ({x}, (mult({y}, {z})))) f>);
+  ("Comm", <f
+    forall x, forall y, [vty_int] plus({x}, {y}) = plus({y}, {x}) f>);
+  ("Inv_def_r", <f
+      forall x, [vty_int] plus ({x}, neg({x})) = zero() f>);
+  ("Inv_def_l", <f
+      forall x, [vty_int] plus (neg({x}), {x}) = zero() f>);
+  ("Unit_def_l", <f
+      forall x, [vty_int] plus (zero(), {x}) = {x} f>);
+  ("Assoc",
+      <f forall x, forall y, forall z, 
+        [vty_int] (plus (plus ({x}, {y}), {z})) = 
+          (plus ({x}, (plus({y}, {z})))) f>)
+  ].
+Proof.
+  reflexivity.
+Qed.
+
+End IntCtx.
